Logic/Modal/Standard/Kripke/GL/Completeness2.lean
@@ -1,0 +1,401 @@
+import Logic.Modal.Standard.Deduction
+import Logic.Modal.Standard.ConsistentTheory
+import Logic.Modal.Standard.Kripke.Semantics
+import Logic.Modal.Standard.Kripke.GL.Completeness
+
+namespace LO.Modal.Standard
+
+variable {α : Type u} [Inhabited α] [DecidableEq α]
+
+
+namespace Formula
+
+variable {p q r : Formula α}
+
+/-- Supplemental subformulas finset for completeness of `𝐆𝐋` -/
+abbrev GLSubformulas (p : Formula α) : Finset (Formula α) := (𝒮 p) ∪ ((𝒮 p).image (complement ·))
+prefix:70 "𝒮⁻ " => Formula.GLSubformulas
+
+namespace GLSubformulas
+
+lemma mem_of_mem_box (h : □q ∈ 𝒮⁻ p) : q ∈ 𝒮⁻ p := by
+  simp_all [GLSubformulas];
+  rcases h with h | ⟨r, _, hr₂⟩;
+  . aesop;
+  . have := complement_box hr₂; subst this;
+    aesop;
+
+lemma mem_of_mem_and (h : q ⋏ r ∈ 𝒮⁻ p) : q ∈ 𝒮⁻ p ∧ r ∈ 𝒮⁻ p := by
+  simp_all [GLSubformulas];
+  rcases h with h | ⟨s, _, hr₂⟩;
+  . aesop;
+  . have := complement_and hr₂; subst this; aesop;
+
+lemma mem_of_mem_and₁ (h : q ⋏ r ∈ 𝒮⁻ p) : q ∈ 𝒮⁻ p := mem_of_mem_and h |>.1
+
+lemma mem_of_mem_and₂ (h : q ⋏ r ∈ 𝒮⁻ p) : r ∈ 𝒮⁻ p := mem_of_mem_and h |>.2
+
+lemma mem_of_mem_or (h : q ⋎ r ∈ 𝒮⁻ p) : q ∈ 𝒮⁻ p ∧ r ∈ 𝒮⁻ p := by
+  simp_all [GLSubformulas];
+  rcases h with h | ⟨s, _, hr₂⟩;
+  . aesop;
+  . have := complement_or hr₂; subst this; aesop;
+
+lemma mem_of_mem_or₁ (h : q ⋎ r ∈ 𝒮⁻ p) : q ∈ 𝒮⁻ p := mem_of_mem_or h |>.1
+
+lemma mem_of_mem_or₂ (h : q ⋎ r ∈ 𝒮⁻ p) : r ∈ 𝒮⁻ p := mem_of_mem_or h |>.2
+
+lemma mem_of_mem_imp (h : q ⟶ r ∈ 𝒮⁻ p) : q ∈ 𝒮⁻ p ∧ r ∈ 𝒮⁻ p := by
+  simp_all [GLSubformulas];
+  rcases h with h | ⟨s, _, hr₂⟩;
+  . aesop;
+  . have := complement_imp hr₂; subst this; aesop;
+
+lemma mem_of_mem_imp₁ (h : q ⟶ r ∈ 𝒮⁻ p) : q ∈ 𝒮⁻ p := mem_of_mem_imp h |>.1
+
+lemma mem_of_mem_imp₂ (h : q ⟶ r ∈ 𝒮⁻ p) : r ∈ 𝒮⁻ p := mem_of_mem_imp h |>.2
+
+lemma mem_subformula_of_mem_box (h : □q ∈ 𝒮⁻ p) : □q ∈ 𝒮 p := by
+  simp [GLSubformulas] at h;
+  rcases h with h | ⟨r, _, hr₂⟩;
+  . assumption;
+  . have := complement_box hr₂; subst this; simpa;
+
+lemma mem_subformula_of_mem_and (h : q ⋏ r ∈ 𝒮⁻ p) : q ⋏ r ∈ 𝒮 p := by
+  simp [GLSubformulas] at h;
+  rcases h with h | ⟨s, _, hr₂⟩;
+  . assumption;
+  . have := complement_and hr₂; subst this; simpa;
+
+lemma mem_subformula_of_mem_or (h : q ⋎ r ∈ 𝒮⁻ p) : q ⋎ r ∈ 𝒮 p := by
+  simp [GLSubformulas] at h;
+  rcases h with h | ⟨s, _, hr₂⟩;
+  . assumption;
+  . have := complement_or hr₂; subst this; simpa;
+
+lemma mem_subformula_of_mem_imp (h : q ⟶ r ∈ 𝒮⁻ p) : q ⟶ r ∈ 𝒮 p := by
+  simp [GLSubformulas] at h;
+  rcases h with h | ⟨s, _, hr₂⟩;
+  . assumption;
+  . have := complement_imp hr₂; subst this; simpa;
+
+lemma mem_subformula_of_mem_top (h : ⊤ ∈ 𝒮⁻ p) : ⊤ ∈ 𝒮 p := by
+  simp [GLSubformulas] at h;
+  rcases h with h | ⟨s, _, hr₂⟩;
+  . assumption;
+  . have := complement_top hr₂; subst this; simpa;
+
+end GLSubformulas
+
+end Formula
+
+
+
+structure Theory.Complete (T : Theory α) (p : Formula α) : Prop where
+  subset_cf : T ⊆ 𝒮⁻ p
+  whichone : ∀ q ∈ 𝒮 p, (q ∈ T) ∨ (-q ∈ T)
+
+namespace Theory
+
+variable {p : Formula α} {T : Theory α}
+-- variable (T_consis : (Λ)-Consistent T) (T_subset : T ⊆ 𝒮⁻ p)
+
+lemma complete_lindenbaum : ∃ Z, (Λ)-Consistent Z ∧ Z.Complete p ∧ T ⊆ Z := by sorry;
+
+lemma not_mem_of_mem_neg (T_consis : (Λ)-Consistent T) (h : ~p ∈ T) : p ∉ T := by
+  by_contra hC;
+  have : [p, ~p] ⊬[Λ]! ⊥ := (Theory.def_consistent.mp T_consis) [p, ~p] (by simp_all);
+  have : [p, ~p] ⊢[Λ]! ⊥ := System.bot_of_mem_either! (p := p) (Γ := [p, ~p]) (by simp) (by simp);
+  contradiction;
+
+end Theory
+
+
+
+structure CompleteConsistentTheory (Λ : DeductionParameter α) (p : Formula α) where
+  theory : Theory α
+  consistent : (Λ)-Consistent theory
+  complete : theory.Complete p
+
+alias CCT := CompleteConsistentTheory
+
+namespace CompleteConsistentTheory
+
+open System
+
+variable {Λ : DeductionParameter α}
+
+lemma lindenbaum (p : Formula α) (consisT : (Λ)-Consistent T) : ∃ Ω : CCT Λ p, (T ⊆ Ω.theory) := by
+  obtain ⟨Z, Z_consis, Z_complete, Z_subset_T⟩ := Theory.complete_lindenbaum (α := α) (Λ := Λ);
+  use ⟨Z, Z_consis, Z_complete⟩;
+
+variable {p : Formula α}
+variable {Ω Ω₁ Ω₂ : CCT Λ p}
+
+lemma mem_compl_of_not_mem (hs : q ∈ 𝒮 p) (h : q ∉ Ω.theory) : -q ∈ Ω.theory := by
+  have := Ω.complete.whichone q (by aesop);
+  aesop;
+
+lemma mem_of_not_mem_compl (hs : q ∈ 𝒮 p) (h : -q ∉ Ω.theory) : q ∈ Ω.theory := by
+  have := Ω.complete.whichone q (by aesop);
+  aesop;
+
+lemma membership_iff (hq : q ∈ 𝒮 p) : (q ∈ Ω.theory) ↔ (Ω.theory *⊢[Λ]! q) := by
+  constructor;
+  . intro h; exact Context.by_axm! h;
+  . intro hp;
+    suffices ~q ∉ Ω.theory by
+      apply or_iff_not_imp_right.mp $ ?_;
+      assumption;
+      have := Ω.complete.whichone q hq;
+      by_cases n : q.negated;
+      . rw [Formula.eq_complement_negated n] at this; simp_all;
+      . rw [Formula.eq_complement_not_negated n] at this; assumption;
+    by_contra hC;
+    have hnp : Ω.theory *⊢[Λ]! ~q := Context.by_axm! hC;
+    have := neg_mdp! hnp hp;
+    have := Ω.consistent;
+    contradiction;
+
+lemma mem_verum (h : ⊤ ∈ 𝒮 p) : ⊤ ∈ Ω.theory := by
+  apply membership_iff h |>.mpr;
+  exact verum!;
+
+@[simp] lemma mem_falsum : ⊥ ∉ Ω.theory := Theory.not_mem_falsum_of_consistent Ω.consistent
+
+lemma unprovable_falsum (h : ⊥ ∈ 𝒮 p) : Ω.theory *⊬[Λ]! ⊥ := by apply membership_iff (by assumption) |>.not.mp; simp
+
+lemma iff_mem_neg (hq : ~p ∈ 𝒮 p) : (~q ∈ Ω.theory) ↔ (q ∉ Ω.theory) := by
+  constructor;
+  . intro hnp;
+    by_contra hp;
+    sorry;
+  . intro hp;
+    sorry;
+
+lemma iff_mem_and (hq : (q ⋏ r) ∈ 𝒮 p) : ((q ⋏ r) ∈ Ω.theory) ↔ (q ∈ Ω.theory) ∧ (r ∈ Ω.theory) := by
+  constructor;
+  . intro hpq;
+    replace hpq := membership_iff (by assumption) |>.mp hpq;
+    constructor;
+    . apply membership_iff (by aesop) |>.mpr;
+      exact and₁'! hpq;
+    . apply membership_iff (by aesop) |>.mpr;
+      exact and₂'! hpq;
+  . rintro ⟨hp, hq⟩;
+    apply membership_iff (by aesop) |>.mpr;
+    exact and₃'! (membership_iff (by aesop) |>.mp hp) (membership_iff (by aesop) |>.mp hq);
+
+lemma iff_mem_or (hq : (q ⋎ r) ∈ 𝒮 p) : ((q ⋎ r) ∈ Ω.theory) ↔ (q ∈ Ω.theory) ∨ (r ∈ Ω.theory) := by
+  constructor;
+  . intro hpq;
+    replace hpq := membership_iff (by assumption) |>.mp hpq;
+    by_contra hC; push_neg at hC;
+    have ⟨hq, hr⟩ := hC;
+    replace hq := membership_iff (by sorry) |>.mp $ @iff_mem_neg α _ Λ p Ω q (by sorry) |>.mpr hC.1;
+    replace hr := membership_iff (by sorry) |>.mp $ @iff_mem_neg α _ Λ p Ω r (by sorry) |>.mpr hC.2;
+    have : Ω.theory *⊢[Λ]! ⊥ := or₃'''! (neg_equiv'!.mp hq) (neg_equiv'!.mp hr) hpq;
+    exact Ω.consistent this;
+  . rintro (hp | hq);
+    . apply membership_iff (by aesop) |>.mpr;
+      exact or₁'! (membership_iff (by aesop) |>.mp hp);
+    . apply membership_iff (by aesop) |>.mpr;
+      exact or₂'! (membership_iff (by aesop) |>.mp hq);
+
+lemma iff_mem_imp (hq : (q ⟶ r) ∈ 𝒮 p) : ((q ⟶ r) ∈ Ω.theory) ↔ (q ∈ Ω.theory) → (r ∈ Ω.theory) := by
+  constructor;
+  . intro hpq;
+    sorry;
+  . rintro hqr;
+    apply membership_iff (by aesop) |>.mpr;
+    sorry;
+
+end CompleteConsistentTheory
+
+namespace Kripke
+
+open Formula
+
+variable {p q : Formula α}
+
+abbrev GLCompleteFrame {p : Formula α} (h : 𝐆𝐋 ⊬! p) : Kripke.FiniteFrame where
+  World := CCT 𝐆𝐋 p
+  World_finite := by
+    sorry;
+  World_nonempty := by
+    have : (𝐆𝐋)-Consistent {~p} := Theory.unprovable_iff_singleton_neg_consistent.mp h;
+    obtain ⟨Ω, hΩ⟩ := CompleteConsistentTheory.lindenbaum p this;
+    exact ⟨Ω⟩;
+  Rel X Y :=
+    (∀ q ∈ □''⁻¹(𝒮 p), □q ∈ X.theory → (q ∈ Y.theory ∧ □q ∈ Y.theory)) ∧
+    (∃ r ∈ □''⁻¹(𝒮 p), □r ∉ X.theory ∧ □r ∈ Y.theory)
+
+namespace GLCompleteFrame
+
+variable {p : Formula α} {h : 𝐆𝐋 ⊬! p}
+
+lemma irreflexive : Irreflexive (GLCompleteFrame h).Rel := by simp [Irreflexive];
+
+lemma transitive : Transitive (GLCompleteFrame h).Rel := by
+  simp;
+  rintro X Y Z ⟨RXY, ⟨r, _, _, _⟩⟩ ⟨RYZ, _⟩;
+  constructor;
+  . rintro q hq₁ hq₂;
+    exact RYZ q hq₁ $ RXY q hq₁ hq₂ |>.2;
+  . use r;
+    refine ⟨by assumption, by assumption, ?_⟩;
+    exact RYZ r (by assumption) (by assumption) |>.2;
+
+end GLCompleteFrame
+
+abbrev GLCompleteModel (h : 𝐆𝐋 ⊬! p) : Kripke.Model α where
+  Frame := GLCompleteFrame h
+  Valuation X a := (atom a) ∈ X.theory
+
+open Formula.Kripke
+open CompleteConsistentTheory
+
+open System System.FiniteContext in
+private lemma GL_truthlemma.lemma1
+  {q : Formula α}
+  {X : Theory α} (X_consistent : (𝐆𝐋)-Consistent X) (h : □q ∉ X) : (𝐆𝐋)-Consistent ({□q, ~q} ∪ (□''⁻¹X ∪ □''□''⁻¹X)) := by
+  by_contra hC;
+  obtain ⟨Γ, hΓ₁, hΓ₂⟩ := Context.provable_iff.mp hC;
+  have := toₛ! hΓ₂;
+  have : 𝐆𝐋 ⊢! ⋀(Γ.remove (~q)) ⋏ ~q ⟶ ⊥ := imply_left_remove_conj! (p := ~q) this;
+  have : 𝐆𝐋 ⊢! ⋀(Γ.remove (~q)) ⟶ ~q ⟶ ⊥ := and_imply_iff_imply_imply'!.mp this;
+  have : 𝐆𝐋 ⊢! ⋀(Γ.remove (~q)) ⟶ q := imp_trans''! this $ imp_trans''! (and₂'! neg_equiv!) dne!
+  have : 𝐆𝐋 ⊢! ⋀((Γ.remove (~q)).remove (□q)) ⋏ □q ⟶ q := imply_left_remove_conj! (p := □q) this;
+  have : 𝐆𝐋 ⊢! ⋀((Γ.remove (~q)).remove (□q)) ⟶ (□q ⟶ q) := and_imply_iff_imply_imply'!.mp this;
+  have : 𝐆𝐋 ⊢! □(⋀(Γ.remove (~q)).remove (□q)) ⟶ □(□q ⟶ q) := imply_box_distribute'! this;
+  have : 𝐆𝐋 ⊢! □(⋀(Γ.remove (~q)).remove (□q)) ⟶ □q := imp_trans''! this axiomL!;
+  have : 𝐆𝐋 ⊢! ⋀□'(Γ.remove (~q)).remove (□q) ⟶ □q := imp_trans''! collect_box_conj! this;
+  have : (□'(Γ.remove (~q)).remove (□q)) ⊢[𝐆𝐋]! □q := provable_iff.mpr this;
+  sorry;
+
+open Formula MaximalConsistentTheory in
+lemma GL_truthlemma₂
+  {p : Formula α} (h : 𝐆𝐋 ⊬! p) {X : (GLCompleteModel h).World}
+  {q : Formula α} (h_sub : q ∈ 𝒮⁻ p) :
+  Satisfies (GLCompleteModel h) X q ↔ q ∈ X.theory := by
+  induction q using Formula.rec' generalizing X with
+  | hbox q ih =>
+    constructor;
+    . contrapose;
+      intro h;
+      have := @GL_truthlemma.lemma1 α _ q X.theory X.consistent h;
+      obtain ⟨Y, hY⟩ := CompleteConsistentTheory.lindenbaum p this;
+      simp [Set.insert_subset_iff] at hY;
+      have ⟨⟨hY₁, hY₂⟩, hY₃, hY₄⟩ := hY;
+      simp [Satisfies];
+      use Y;
+      constructor;
+      . intro r hr₁ hr₂;
+        constructor;
+        . apply hY₃; exact hr₂;
+        . apply hY₄; exact hr₂;
+      . use q;
+        refine ⟨?_, ?_, ?_, ?_⟩;
+        . exact GLSubformulas.mem_subformula_of_mem_box h_sub;
+        . assumption;
+        . assumption;
+        . apply @ih Y (GLSubformulas.mem_of_mem_box h_sub) |>.not.mpr;
+          apply Theory.not_mem_of_mem_neg Y.consistent (by aesop);
+    . intro h Y RXY;
+      apply ih (X := Y) (GLSubformulas.mem_of_mem_box h_sub) |>.mpr
+      simp [Frame.Rel'] at RXY;
+      exact RXY.1 q (GLSubformulas.mem_subformula_of_mem_box h_sub) h |>.1;
+  | hverum =>
+    simp [Satisfies];
+    exact CompleteConsistentTheory.mem_verum (GLSubformulas.mem_subformula_of_mem_top h_sub);
+  | hfalsum => simp [Satisfies];
+  | hatom => simp [Satisfies];
+  | hand q r ihq ihr =>
+    constructor;
+    . intro h; simp [Satisfies] at h;
+      have ⟨hq₁, hq₂⟩ := GLSubformulas.mem_of_mem_and h_sub;
+      apply iff_mem_and (GLSubformulas.mem_subformula_of_mem_and h_sub) |>.mpr;
+      constructor;
+      . apply ihq hq₁ |>.mp h.1;
+      . apply ihr hq₂ |>.mp h.2;
+    . intro h;
+      have ⟨hq₁, hq₂⟩ := GLSubformulas.mem_of_mem_and h_sub;
+      constructor;
+      . apply ihq hq₁ |>.mpr;
+        exact CompleteConsistentTheory.iff_mem_and (GLSubformulas.mem_subformula_of_mem_and h_sub) |>.mp h |>.1;
+      . apply ihr hq₂ |>.mpr;
+        exact CompleteConsistentTheory.iff_mem_and (GLSubformulas.mem_subformula_of_mem_and h_sub) |>.mp h |>.2;
+  | hor q r ihq ihr =>
+    constructor;
+    . intro h; simp [Satisfies] at h;
+      have ⟨hq₁, hq₂⟩ := GLSubformulas.mem_of_mem_or h_sub;
+      apply iff_mem_or (GLSubformulas.mem_subformula_of_mem_or h_sub) |>.mpr;
+      rcases h with h | h;
+      . left; apply ihq (X := X) hq₁ |>.mp h;
+      . right; apply ihr (X := X) hq₂ |>.mp h;
+    . intro h;
+      have ⟨hq₁, hq₂⟩ := GLSubformulas.mem_of_mem_or h_sub;
+      rcases CompleteConsistentTheory.iff_mem_or (GLSubformulas.mem_subformula_of_mem_or h_sub) |>.mp h with h | h;
+      . left; apply ihq (X := X) hq₁ |>.mpr; exact h;
+      . right; apply ihr (X := X) hq₂ |>.mpr; exact h;
+  | himp q r ihq ihr =>
+    have := Subformulas.mem_imp₁ $ GLSubformulas.mem_subformula_of_mem_imp h_sub;
+    have := Subformulas.mem_imp₂ $ GLSubformulas.mem_subformula_of_mem_imp h_sub;
+    constructor;
+    . contrapose;
+      intro h;
+      sorry;
+    . contrapose;
+      intro h; simp [Satisfies] at h;
+      obtain ⟨hq, hr⟩ := h;
+      replace hq : X.theory *⊢[𝐆𝐋]! q := CompleteConsistentTheory.membership_iff (by assumption) |>.mp
+        $ ihq (GLSubformulas.mem_of_mem_imp₁ h_sub) |>.mp hq;
+      replace hr : -r ∈ X.theory := mem_compl_of_not_mem (by assumption) $ ihr (GLSubformulas.mem_of_mem_imp₂ h_sub) |>.not.mp hr;
+      by_cases n : r.negated;
+      . rw [Formula.eq_complement_negated n] at *;
+        replace hr := CompleteConsistentTheory.membership_iff (by assumption) |>.mp hr;
+        apply Theory.not_mem_of_mem_neg X.consistent;
+        apply CompleteConsistentTheory.membership_iff (by sorry) |>.mpr;
+        sorry;
+      . rw [Formula.eq_complement_not_negated n] at *;
+
+        apply Theory.not_mem_of_mem_neg X.consistent;
+        sorry;
+    /-
+    . intro h; simp [Satisfies] at h;
+      have ⟨hq₁, hq₂⟩ := GLSubformulas.mem_of_mem_imp hq;
+      apply iff_mem_imp (GLSubformulas.mem_subformula_of_mem_imp hq) |>.mpr;
+      intro hq;
+      apply ihr hq₂ |>.mp $ ihr hq₂ |>.mpr (by aesop);
+    . intro h hhq;
+      have ⟨hq₁, hq₂⟩ := GLSubformulas.mem_of_mem_imp hq;
+      have := @CompleteConsistentTheory.iff_mem_imp α _ 𝐆𝐋 p X q r ?_ |>.mp h ?_;
+      apply ihr ?_ |>.mpr;
+      assumption;
+      . assumption;
+      . exact GLSubformulas.mem_subformula_of_mem_imp hq
+      . simp_all;
+    -/
+  | hneg q ihq =>
+    constructor;
+    . intro h; simp [Satisfies] at h;
+      sorry;
+    . intro h hnq;
+      sorry;
+
+private lemma GL_completeAux : TransitiveIrreflexiveFrameClass.{u}ꟳ# ⊧ p → 𝐆𝐋 ⊢! p := by
+  contrapose;
+  intro h;
+  apply exists_finite_frame.mpr;
+  use (GLCompleteFrame h);
+  constructor;
+  . exact ⟨GLCompleteFrame.transitive, GLCompleteFrame.irreflexive⟩;
+  . simp [Formula.Kripke.ValidOnFrame, Formula.Kripke.ValidOnModel];
+    have ⟨X, hX⟩ := lindenbaum (Λ := 𝐆𝐋) (T := {~p}) (p := p) (Theory.unprovable_iff_singleton_neg_consistent.mp h);
+    use (GLCompleteModel h).Valuation, X;
+    apply GL_truthlemma₂ (h := h) (by simp) |>.not.mpr;
+    apply Theory.not_mem_of_mem_neg X.consistent (by aesop);
+
+end Kripke
+
+end LO.Modal.Standard
